One more test

state/Backtranslation.STLCToTargetLang.fst
@@ -294,6 +294,24 @@ let progr_passing_encapsulated_to_callback_test rp rs f =
   downgrade_val (f cb);
   ()
 
+val progr_passing_private_to_callback_test:
+  ctx:(elab_typ default_spec (TArr (TArr TUnit TUnit) TUnit)) ->
+  SST unit
+    (requires (fun h0 -> True))
+    (ensures (fun h0 _ h1 -> True))
+[@expect_failure]
+let progr_passing_private_to_callback_test f =
+  let secret: ref int = sst_alloc #SNat 0 in
+  witness (contains_pred secret);
+  let cb: elab_typ default_spec (TArr TUnit TUnit) = (fun _ ->
+    recall (contains_pred secret);
+    // let h0 = get_heap () in
+    // assume (is_shared secret h0);
+    sst_write #SNat secret (!secret + 1);
+    raise_val ()) in
+  downgrade_val (f cb);
+  ()
+
 val progr_getting_callback_test:
   rp: ref int ->
   rs: ref (ref int) ->
